\documentclass[a4paper,12pt]{article}

%%%%%%%%%%%%%%%%%%%%%%%%%%%%%%%%%%%%%%%%%%%%%%%%%%%%%%%%%%%%%%%%%%%%%%%%%%%%%%%%%%%%%%%%%%%%%%%%%%%%%%%%%%%%%%%%%%%%%%%%%%%%%%%%%%%%%%%%%%%%%%%%%%%%%%%%%%%%%%%%%%%%%%%%%%%%%%%%%%%%%%%%%%%%%%%%%%%%%%%%%%%%%%%%%%%%%%%%%%%%%%%%%%%%%%%%%%%%%%%%%%%%%%%%%%%%

\usepackage{eurosym}
\usepackage{vmargin}
\usepackage{amsmath}
\usepackage{graphics}
\usepackage{epsfig}
\usepackage{enumerate}
\usepackage{multicol}
\usepackage{subfigure}
\usepackage{fancyhdr}
\usepackage{listings}
\usepackage{framed}
\usepackage{graphicx}
\usepackage{amsmath}
\usepackage{chngpage}

%\usepackage{bigints}
\usepackage{vmargin}

% left top textwidth textheight headheight

% headsep footheight footskip

\setmargins{2.0cm}{2.5cm}{16 cm}{22cm}{0.5cm}{0cm}{1cm}{1cm}

\renewcommand{\baselinestretch}{1.3}

\setcounter{MaxMatrixCols}{10}

\begin{document}

\begin{enumerate}

%%%%%%%%%%%%%%%%%%%%%%%%%%%%%%%%%%%%%%%%%%%%%%%%%%%%%%%%%%%%%%%%%%%%%%%%%%%%%%%%%%%%%%%%%%%%%%%%%%%%%%%%%%%%%%%%%%%%%%%%%%%%%%%%%%%%%%%%%%
\item 11 Consider the following model for aggregate claim amounts S:
\[S = X1 + X2 + \ldots+ XN\]
where the Xi are independent, identically distributed random variables representing individual claim amounts and N is a random variable, independent of the $X_i$ , and representing the number of claims. Let $X$ have mean $\mu_X$ and let $N$ have mean $\mu_N$ and
variance $\sigma^2_N$.
\begin{enumerate}[(a)]
\item Show that
\[E(SN) = X (2N  2N )\]
by considering expected values conditional on the value of N. 
\item Hence derive an expression for the covariance between $S$ and $N$. 
\end{enumerate}
\end{enumerate}


%%%%%%%%%%%%%%%%%%%%%%%%%%%%%%%%%%%%%%%%%%%%%%%%%%%%%%%%%%%%%%%%%%%%%%%%%%%%%%%%%%%%%%%%%%%%%%%%%%%%%%%%%%%%%%%%%%%%%%%%%%%%%%%%%%%%%%%%%%
\item E(S) = E(NX) = NX
\begin{eqnarray*}
\operatornmae{Cov}(S,N) &=& E(SN) - E(S)E(N)\\
&=& \mu_x (\mu^2_N + \sigma^2_N) \;-\; (\mu_N \mu_X)\mu_N \\
&=& \mu_X \sigma^2_N
\end{eqnarray*}

\end{itemize}
\newpage


%%%%%%%%%%%%%%%%%%%%%%%%%%%%%%%%%%%%%%%%%%%%%%%%%%%%%%%%%%555555


11
(i) 
$P(T < x) = 1 - exp(-\lambda x)$ so $X \sim bin(n , 1 - exp(-\lambda t_{0} ))$
(ii) (a)

\[ L(\lambda ) \proportional   (1 - exp(-\lambda t_{0} ))^x [exp(-\lambda t_{0} ) ]^{n-x}\]

\begin{eqnarray*}
\mathcal{l}(\lambda) &=& x\log(1 - exp(-\lambda t_{0} )) + (n - x)\log[exp(-\lambda t_{0} )] + \mbox{constant}\\
&=& x\log(1 - exp(-\lambda t_{0} )) - (n - x)\lambda t_0 + \mbox{constant}\\
\end{eqnarray*}
%-----------------------------------%
(b)

\begin{eqnarray*}
\frac{\partial {\mathcal{l}}{\partial \lambda} 
&=& xt_0 exp(-\lambda t_{0} ) /(1 - exp(-\lambda t_{0} )) - (n - x)t_0\\
&=& xt_0 \frac{1 + exp(-\lambda t_{0} ) }{(1 - exp(-\lambda t_{0} ))} - nt_0\\
&=& \frac{xt_0 }{(1 - exp(-\lambda t_{0} ) }  - nt_0\\
\end{eqnarray*}

\end{document}
